Re-factor definitions and modules.

src/dafny/smart/Deposit.dfy
@@ -12,187 +12,76 @@
  * under the License.
  */
 
-include "Helpers.dfy"
+include "Trees.dfy"
+include "MerkleTrees.dfy"
 
-module DepositSmartContract {
+module DepositTree {
 
-    import opened Helpers
-
-    /** Merkle Binary trees.
-     *
-     *  Values are in a domain `T`.
-     *  
-     *  @param  l   This ghost variable is the level of a node.
-     *              It is 0 for leaves.
-     *  @param  i   The index of a child at a given level.
-     */
-    datatype Node<T> = 
-            Leaf(v: T, ghost l: nat, ghost i: nat)
-        |   Node(v: T, left: Node, right: Node, ghost l: nat, ghost i: nat)
-
-    /**
-     *  Height of a tree.
-     */
-    function height<T>(root : Node<T>) : nat 
-        ensures height(root) >= 1
-        decreases root
-    {
-        match root 
-            //  a leaf, level 0 is a MT of height 1
-            case Leaf(_, _, _) => 1
-            //  A node, level l, is a MT of height h if both children are MTs of height h - 1
-            case Node(_, lc, rc, _, _) => 1 + max(height(lc), height(rc))
-    }
-
-    /**
-     *  We return a sequence of nodes.
-     *
-     *  @note   We may not use a set for collectting the nodes, as it is possible that
-     *          that two nodes in subtrees are equal.
-     */
-    function collectNodes<T>(root : Node<T>) : seq<Node<T>>
-        decreases root
-    {
-        match root 
-            case Leaf(_, _, _) => [ root ] 
-            case Node(_, lc, rc, _, _) =>  [ root ] + collectNodes<T>(lc) + collectNodes<T>(rc) 
-    }
-
-    /**
-     *  We return the leaves as a sequence from left to right.
-     *
-     */
-    function collectLeaves<T>(root : Node<T>) : seq<Node<T>>
-        decreases root
-    {
-        match root 
-            case Leaf(_, _, _) => [ root ] 
-            case Node(_, lc, rc, _, _) =>  
-                collectLeaves<T>(lc) + collectLeaves<T>(rc) 
-    }
-    
-    /**
-     *  Whether the tree defined by a node is a Merkle Tree of height `h`.
-     */
-    predicate isCompleteTree<T>(root : Node<T>) 
-        decreases root
-    {
-        match root 
-            //  A leaf is a complete tree
-            case Leaf(_, _, _) => true
-            //  From a root node, a tree is complete if both children have same height
-            case Node(_, lc, rc, _, _) => 
-                && height(lc) == height(rc) 
-                && isCompleteTree(lc) && isCompleteTree(rc)
-    }
-
-    /**
-     *  Check that the levels in a tree are set according to the height - 1.
-     *
-     */
-    predicate isMerkleLevelTree<T>(root : Node<T>, level: nat) 
-        requires isCompleteTree(root)
-        decreases root
-    {
-        root.l == height(root) - 1
-    }
-    
-    /**
-     *
-     *  Nodes in a Merkle tree can be indexed at each level from 1 to 2^(h - l) - 1.
-     *  @todo   Check from 1 to 2^(h - l) - 1.
-     *  @todo   Write the definition! for now consistently returns true ...
-     */
-    predicate isMerkleIndexedTree<T>(root : Node<T>, level: nat) 
-        requires isCompleteTree(root)
-        decreases root
-    {
-         match root 
-           case Leaf(_, l, i) => true
-           case Node(_, lc, rc, l, i) => true
-    }
-     
-    /**
-     *  Relation between heigth and number of leaves in a complete tree.
-     */
-    lemma {:induction root} completeTreeNumberOfLeaves<T>(root : Node<T>) 
-        requires isCompleteTree(root)
-        ensures |collectLeaves(root)| == power2(height(root) - 1)
-    {   //  Thanks Dafny
-    }
-
-    /**
-     *  Relation between heigth and number of nodes in a complete tree.
-     */
-    lemma {:induction root} completeTreeNumberOfNodes<T>(root : Node<T>) 
-        requires isCompleteTree(root)
-        ensures |collectNodes(root)| == power2(height(root)) - 1
-    {   //  Thanks Dafny
-    }
-
-    //  Trees holding integer attributes
-    type Intnode = Node<int>
+    import opened Trees
+    import opened MerkleTrees
 
     /** 
-     *  Difference between two integers.
+     *  Attribute hash.
+     *
      */
-    function diff(a: int, b : int) : int 
-    {
-        a - b
-    }
+    function hash<T>(a: T, b : T) : T 
 
     /**
      *  Check that a decorated tree correctly stores the diff attribute. 
      */
-    predicate isDecoratedWithDiff(root: Node<int>)
+    predicate isDecoratedWithHash<T>(root: Node<T>)
     {
         match root
             case Leaf(v, _, _) => true
 
-            case Node(v, lc, rc, _, _) => v == diff(lc.v, rc.v)
+            case Node(v, lc, rc, _, _) => v == hash(lc.v, rc.v)
     }
 
     /**
-     *  
+     *  Incremental algorithm.
      */
+    class HashTree {
 
-/*
- * fun init() -> unit:
- *     i: int = 0
- *     while i < TREE_HEIGHT - 1:
- *         zerohashes[i+1] = hash(zerohashes[i], zerohashes[i])
- *         i += 1
- */
+        /*
+        * fun init() -> unit:
+        *     i: int = 0
+        *     while i < TREE_HEIGHT - 1:
+        *         zerohashes[i+1] = hash(zerohashes[i], zerohashes[i])
+        *         i += 1
+        */
 
-/*
- * fun deposit(value: int) -> unit:
- *     assert deposit_count < 2^TREE_HEIGHT - 1
- *     deposit_count += 1
- *     size: int = deposit_count
- *     i: int = 0
- *     while i < TREE_HEIGHT - 1:
- *         if size % 2 == 1:
- *             break
- *         value = hash(branch[i], value)
- *         size /= 2
- *         i += 1
- *     branch[i] = value
- */
+        /*
+        * fun deposit(value: int) -> unit:
+        *     assert deposit_count < 2^TREE_HEIGHT - 1
+        *     deposit_count += 1
+        *     size: int = deposit_count
+        *     i: int = 0
+        *     while i < TREE_HEIGHT - 1:
+        *         if size % 2 == 1:
+        *             break
+        *         value = hash(branch[i], value)
+        *         size /= 2
+        *         i += 1
+        *     branch[i] = value
+        */
 
-/*
- * fun get_deposit_root() -> int:
- *     root: int = 0
- *     size: int = deposit_count
- *     h: int = 0
- *     while h < TREE_HEIGHT:
- *         if size % 2 == 1: # size is odd
- *             root = hash(branch[h], root)
- *         else:             # size is even
- *             root = hash(root, zerohashes[h])
- *         size /= 2
- *         h += 1
- *     return root
- */
+        /*
+        * fun get_deposit_root() -> int:
+        *     root: int = 0
+        *     size: int = deposit_count
+        *     h: int = 0
+        *     while h < TREE_HEIGHT:
+        *         if size % 2 == 1: # size is odd
+        *             root = hash(branch[h], root)
+        *         else:             # size is even
+        *             root = hash(root, zerohashes[h])
+        *         size /= 2
+        *         h += 1
+        *     return root
+        */
+
+} 
+   
 
 
 }
