src/dafny/smart/IntTree.dfy
@@ -1,0 +1,70 @@
+/*
+ * Copyright 2020 ConsenSys AG.
+ *
+ * Licensed under the Apache License, Version 2.0 (the "License"); you may 
+ * not use this file except in compliance with the License. You may obtain 
+ * a copy of the License at http://www.apache.org/licenses/LICENSE-2.0
+ *
+ * Unless required by applicable law or agreed to in writing, software dis-
+ * tributed under the License is distributed on an "AS IS" BASIS, WITHOUT 
+ * WARRANTIES OR CONDITIONS OF ANY KIND, either express or implied. See the 
+ * License for the specific language governing permissions and limitations 
+ * under the License.
+ */
+
+include "Trees.dfy"
+include "MerkleTrees.dfy"
+
+module DiffTree {
+
+    import opened Trees
+    import opened MerkleTrees
+
+    //  Trees holding integer values as attribute.
+    type Intnode = Node<int>
+
+    /** 
+     *  Difference between two integers.
+     *
+     *  @note:  This could be inlined in the predicate
+     *          isDecoratedWithDiff, but we may use another 
+     *          function later, so we factor it out.
+     */
+    function diff(a: int, b : int) : int 
+    {
+        a - b
+    }
+
+    /**
+     *  Check that a decorated tree correctly stores the diff attribute. 
+     */
+    predicate isDecoratedWithDiff(root: Node<int>)
+    {
+        match root
+            case Leaf(v, _, _) => true
+
+            case Node(v, lc, rc, _, _) => v == diff(lc.v, rc.v)
+    }
+
+    /**
+     *  Incremental algorithm.
+     */
+    class IntTree {
+
+        constructor()
+
+        method incrDiffAlgo(root: Node<int>, l: seq<int>, e: int) returns (root' : Node<int>) 
+            requires isCompleteTree(root)
+            requires |l| < |collectLeaves(root)|
+            requires MerkleTrees.treeLeftmostLeavesMatchList(l, root, 0)
+
+            ensures isCompleteTree(root')
+            ensures height(root') == height(root)
+            ensures MerkleTrees.treeLeftmostLeavesMatchList(l + [e], root', 0)
+        {
+
+        }
+
+    } 
+
+}
