src/dafny/smart/MerkleTrees.dfy
@@ -1,0 +1,65 @@
+/*
+ * Copyright 2020 ConsenSys AG.
+ *
+ * Licensed under the Apache License, Version 2.0 (the "License"); you may 
+ * not use this file except in compliance with the License. You may obtain 
+ * a copy of the License at http://www.apache.org/licenses/LICENSE-2.0
+ *
+ * Unless required by applicable law or agreed to in writing, software dis-
+ * tributed under the License is distributed on an "AS IS" BASIS, WITHOUT 
+ * WARRANTIES OR CONDITIONS OF ANY KIND, either express or implied. See the 
+ * License for the specific language governing permissions and limitations 
+ * under the License.
+ */
+
+include "Helpers.dfy"
+include "Trees.dfy"
+
+module MerkleTrees {
+
+    import opened Helpers
+    import opened Trees
+
+    /**
+     *  Check that the levels in a tree are set according to the height - 1.
+     *
+     */
+    predicate isMerkleLevelTree<T>(root : Node<T>, level: nat) 
+        requires isCompleteTree(root)
+        decreases root
+    {
+        root.l == height(root) - 1
+    }
+    
+    /**
+     *
+     *  Nodes in a Merkle tree can be indexed at each level from 1 to 2^(h - l) - 1.
+     *  @todo   Check from 1 to 2^(h - l) - 1.
+     *  @todo   Write the definition! for now consistently returns true ...
+     */
+    predicate isMerkleIndexedTree<T>(root : Node<T>, level: nat) 
+        requires isCompleteTree(root)
+        decreases root
+    {
+         match root 
+           case Leaf(_, l, i) => true
+           case Node(_, lc, rc, l, i) => true
+    }
+     
+    /**
+     *  
+     *  @param  l       A list of elements.
+     *  @param  root    A tree.
+     *  @param  default The default vakue for right-padding the tree leaves.
+     *
+     *  We assume collectLeaves return an indexed from left to right list of leaves.
+     */
+    predicate treeLeftmostLeavesMatchList<T>(l: seq<T>, root: Node<T>, default: T)
+        requires |l| <= |collectLeaves(root)|
+    {
+        forall i:: 
+            0 <= i < |l| ==> l[i] == collectLeaves(root)[i].v
+            && |l| <= i < |collectLeaves(root)|  ==> collectLeaves(root)[i].v == default
+    }
+
+}
